::: {.content-hidden}
$
{{< include macros.tex >}}
$
:::





# Complex Numbers


::: Definition
### Complex Numbers

The set of complex numbers $\C$ is defined as

$$
\C := \R + i \R  := \{x + i y  \divider x, y \in \R \} \,.
$$
For a complex number
$$
z = x + i y  \in \C
$$
we say that

- $x$ is the **real part** of $z$, and denote it by 
$$
x = \Re (z)
$$
- $y$ is the **imaginary part** of $z$, and denote it by 
$$
y = \Im (z)
$$

We say that

- If $\Re z = 0$ then $z$ is a **purely imaginary** number.
- If $\Im z = 0$ then $z$ is a **real** number.

:::


::: Definition
### Addition and multiplication in $\C$   {#definition-addition-C}

Let $z_1,z_2 \in \C$, so that 
$$
z_1 = x_1 + i y_1 \,\,, \quad z_2 = x_2 + i  y_2 \,\, ,
$$
for some $x_1,x_2,y_1,y_2 \in \R$:

1. The sum of $z_1$ and
$z_2$ is
$$
z_1 + z_2 :=\left(x_{1}+x_{2}\right) + i  \left(y_{1}+y_{2}\right) \,.
$$ 

2. The multiplication of $z_1$ and $z_2$ is 
\begin{align*}
z_1 \cdot z_2 := \left(x_{1} \cdot x_{2} - y_{1} \cdot y_{2}\right) + i \left(x_{1} \cdot y_{2} + x_{2} \cdot y_{1} \right) \,,
\end{align*}

:::



::: Example

**Question.** Compute $zw$, where
$$
z =  -2+3 i \,, \quad w = 1- i \,.
$$

**Solution.** Using the definition we compute
\begin{align*}
z \cdot w & = (-2+3 i) \cdot (1 -  i) \\ 
            & = (-2-(-3))+(2+3) i \\
            & = 1 + 5 i \, .
\end{align*}
Alternatively, we can proceed formally: We just need to recall that
$i^2$ has to be replaced with $-1$:
\begin{align*}
z \cdot w & = (-2+3 i) \cdot (1 -  i) \\ 
            & = - 2 + 2i + 3i - 3 i^2  \\
            & = (-2  + 3 ) + (  2 + 3 ) i \\
            & = 1 + 5 i \, .
\end{align*}

:::



::: Proposition
### Additive inverse in $\C$  {#proposition-C-additive-inverse}

The neutral element of addition in $\C$ is the number
$$
0 := 0 + 0 i \,.
$$
For any $z = x + i y \in \C$, the unique additive inverse is given by
$$
- z := -x - i y \,.
$$


:::


::: Proposition
### Multiplicative inverse in $\C$  {#proposition-C-multiplicative-inverse-bis}

The neutral element of multiplication in $\C$ is the number
$$
1 := 1 + 0 i \,.
$$
For any $z = x + i y \in \C$, the unique multiplicative inverse is given by 
$$
z^{-1} := \frac{x}{x^{2}+y^{2}}+ i \, \frac{-y}{x^{2}+y^{2}} \,.
$$

:::


::: Proof
It is immediate to check that $1$ is the neutral element of 
multiplication in $\C$. For the remaining part of the statement, set
$$
w := \frac{x}{x^{2}+y^{2}}+ i \, \frac{-y}{x^{2}+y^{2}} \,.
$$
We need to check that $z \cdot w = 1$
\begin{align*}
z \cdot w & = (x+i y) \cdot \left(\frac{x}{x^{2}+y^{2}}+ i \, \frac{-y}{x^{2}+y^{2}} \right) \\
& = \left(\frac{x^{2}}{x^{2}+y^{2}} - \frac{y \cdot(-y)}{x^{2}+y^{2}}\right) + i \, \left(\frac{x \cdot(-y)}{x^{2}+y^{2}}+\frac{x y}{x^{2}+y^{2}}\right) \\
& =1 \,,
\end{align*}
so indeed $z^{-1}=w$.

:::








::: Example

**Question.** Let $z = 3 + 2 i$. Compute $z^{-1}$. 


**Solution.** By the formula in Propostion \ref{proposition-C-multiplicative-inverse-bis} we immediately get
$$
z^{-1} = \frac{3}{3^{2}+2^{2}} +  \, \frac{-2}{3^{2}+2^{2}} \, i = 
\frac{3}{13}-\frac{2}{13} \, i  \,.
$$
Alternatively, we can proceed formally:
\begin{align*}
(3+2 i)^{-1} & = \frac{1}{3+2 i} \\ 
             & = \frac{1}{3+2 i} \, \frac{3-2 i}{3-2 i} \\
             & = \frac{3-2 i}{3^2+2^2} \\
             & = \frac{3}{13}-\frac{2}{13} i  \,,
\end{align*}
and obtain the same result.
:::



::: Theorem 

$(\C,+, \cdot)$ is a field.

:::



::: Example

**Question.** Let $w=1+i$ and $z=3-i$. Compute $\frac{w}{z}$.

**Solution.** We compute $w/z$ using the two options we have:

1. Using the formula for the inverse from Proposition \ref{proposition-C-multiplicative-inverse-bis} we compute
\begin{align*}
z^{-1} & = \frac{x}{x^{2}+y^{2}} + i \, \frac{-y}{x^{2}+y^{2}} \\
       & = \frac{3}{3^2 + 1^2} - i \, \frac{-1}{3^2 + 1^2} \\
       & = \frac{3}{10} + \frac{1}{10} \, i
\end{align*}
and therefore
\begin{align*}
\frac{w}{z} & = w \cdot z^{-1} \\
            & = (1 + i) \, \left(  \frac{3}{10} + \frac{1}{10} \, i \right) \\
            & = \left(\frac{3}{10}-\frac{1}{10}\right)+\left(\frac{1}{10}+\frac{3}{10}\right) i \\
            & = \frac{2}{10}+\frac{4}{10} i \\
            & = \frac{1}{5}+\frac{2}{5} i
\end{align*}

2. We proceed formally, using the 
multiplication by $1$ trick. We have
\begin{align*}
\frac{w}{z} & = \frac{1+i}{3-i}  \\
            & = \frac{1+i}{3-i} \frac{3+i}{3+i} \\
            & = \frac{3-1+(3+1) i}{3^2+1^2} \\
            & =\frac{2}{10}+\frac{4}{10} i \\
            & = \frac{1}{5}+\frac{2}{5} i
\end{align*}


:::



::: Definition 
### Complex conjugate

Let $z=x+iy$. We call the **complex conjugate** of $z$, denoted by $\bar{z}$, the complex number

$$
\bar{z}=x- i y \, .
$$


:::




::: Theorem 

For all $z_1, z_2 \in \mathbb{C}$ it holds:

- $\overline{z_1 +  z_2 }=\overline{z_1}+\overline{z_2}$

- $\overline{z_1 \cdot z_2}=\overline{z_1} \cdot \overline{z_2}$ 

:::





## The complex plane


![A point $z = x + iy \in \C$ can be represented on the complex plane by the point of coordinates $(x,y)$. The distance between $z$ and $0$ is given by $|z| = \sqrt{z^2 + y^2}$. ](/images/complex_plane.png){#fig-complex-plane width=30%}


::: Definition
### Modulus

The **modulus** of a complex number $z=x+i y$ is defined by
$$
|z|: = \sqrt{x^{2}+y^{2}} \,.
$$
:::



::: Definition
### Distance in $\C$

Given $z_1,z_2 \in \C$, we define the **distance** between $z_1$ and 
$z_2$ as the quantity
$$
|z_1 - z_2| \,.
$$

:::


::: Theorem

Given $z_1,z_2 \in \C$, we have
$$
|z_1 - z_2|  = \sqrt{ (x_1 - x_2)^2 + (y_1 - y_2)^2 }  \,.
$$

:::



::: Example

**Question.** Compute the distance between 
$$
z = 2-4 i \,, \quad 
w = -5+i \,.
$$ 

**Solution.**
The distance is
\begin{align*}
|z- w|  & = |(2-4 i)-(-5+i)| \\
        & = |7-5 i| \\
        & =\sqrt{7^{2}+(-5)^{2}} \\
        & =\sqrt{74}
\end{align*}

:::



::: Theorem 

Let $z, z_{1}, z_{2} \in \C$. Then

1. $\left|z_1 \cdot z_2\right|=\left|z_{1}\right|\left|z_{2}\right|$

2. $\left|z^{n}\right|=|z|^{n}$ for all $n \in \N$

3. $z \cdot \bar{z}=|z|^{2}$

:::



::: Theorem 
### Triangle inequality in $\C$ 

For all $x, y, z \in \C$,

1. $|x+y| \leq|x|+|y|$

2. $|x-z| \leq|x-y|+|y-z|$

:::



## Polar coordinates

![Polar coordinates $(\rho,\theta)$ for the complex number $z \in \C$. ](/images/polar_coordinates.png){#fig-polar-coordinates width=30%}


::: Definition 
### Argument

Let $z \in \C$. The angle $\theta$ between the line connecting the origin and $z$ and the positive real axis is called the **argument** of $z$, and is denoted by
$$
\theta := \arg (z) \,.
$$

:::



::: Example 
We have the following arguments:
\begin{align*}
& \arg (1) = 0  & \quad & \arg (i) = \frac{\pi}{2}  \\
& \arg (-1) = \pi   & \quad & \arg (-i) = -\frac{\pi}{2}  \\
& \arg (1+i)=\frac{1}{4} \pi & \quad &  \arg (-1-i)=-\frac{3}{4} \pi
\end{align*}

:::



::: Theorem  
### Polar coordinates {#theorem-polar-coordinates}

Let $z \in \C$ with $z = x + i y$ and $z \neq 0$. Then
$$
x = \rho \cos(\theta) \,, \quad y = \rho \sin(\theta) \,,
$$
where 
$$
\rho := |z| = \sqrt{x^2 + y^2} \,, \quad 
\theta := \arg(z) \,.
$$


:::





::: Definition 
### Trigonometric form

Let $z \in \mathbb{C}$. The trigonometric form of $z$ is
$$
z = |z| \left[ \cos (\theta)+i \sin (\theta) \right] \,,
$$
where $\theta = \arg(z)$.
:::





::: {.Example   #example-trigonometric-form} 

**Question.** Suppose that $z \in \C$ has polar coordinates
$$
\rho = \sqrt{8}\,, \quad   \theta = \frac{3}{4} \pi \,.
$$ 
Therefore, the trigonometric form of $z$ is
$$
z = \sqrt{8}  \left[ \cos \left( \frac{3}{4} \pi \right) + i \sin \left( \frac{3}{4} \pi \right)   \right] \,.
$$
Write $z$ in cartesian form.

**Solution.** We have
\begin{gather*}
x = \rho \cos (\theta) = \sqrt{8} \cos \left( \frac{3}{4} \pi \right) = - \sqrt{8} \cdot \frac{\sqrt{2}}{2} = -2 \\
y = \rho \sin (\theta) = \sqrt{8} \sin \left( \frac{3}{4} \pi \right) = \sqrt{8} \cdot  \frac{\sqrt{2}}{2} = 2 \,.
\end{gather*}
Therefore, the cartesian form of $z$ is
$$
z = x + i y = - 2 + 2 i \,.
$$

:::


::: Corollary
### Computing $\arg(z)$   {#corollary-arg}

Let $z \in \C$ with $z = x + i y$ and $z \neq 0$. Then
$$
\arg(z) = 
\begin{cases}
\arctan \left(  \dfrac{y}{x}   \right)  &  \,\, \mbox{ if }  x>0 \\
\arctan \left(  \dfrac{y}{x}   \right) + \pi   &  \,\, \mbox{ if }  x<0\,\, \mbox{and} \,\, y \geq 0 \\
\arctan \left(  \dfrac{y}{x}   \right) - \pi   &  \,\, \mbox{ if }  x<0\,\, \mbox{and} \,\, y < 0 \\
\dfrac{\pi}{2}    &  \,\, \mbox{ if }  x=0\,\, \mbox{and} \,\, y > 0 \\
-\dfrac{\pi}{2}    &  \,\, \mbox{ if }  x=0\,\, \mbox{and} \,\, y < 0 \\
\end{cases}
$$
where $\arctan$ is the inverse of $\tan$.

:::


![The definition of $\arg(z)$ depends on the position of $z$ in the complex plane.](/images/argument_1.png){#fig-argument-1 width=35%}


::: Example 

**Question.** Compute the arguments of the complex numbers 
$$
z = 3+4 i\,, \quad \bar{z} = 3-4 i \,, \quad  - \bar{z} = -3+4 i \,, \quad - z= -3-4 i \,.
$$ 

**Solution.** Using the formula for $\arg$ in Corollary \ref{corollary-arg} we have
\begin{align*}
\arg (3+4 i) & =\arctan \left(\frac{4}{3}\right) \\
\arg (3-4 i) & =\arctan \left(-\frac{4}{3}\right) = -\arctan \left(\frac{4}{3}\right)  \\
\arg (-3+4 i) & = \arctan \left(-\frac{4}{3}\right) + \pi = - \arctan \left(\frac{4}{3}\right) + \pi \\
\arg (-3-4 i) & = \arctan \left(\frac{4}{3}\right) - \pi
\end{align*}

:::




## Exponential form

::: Theorem 
### Euler's identity   {#theorem-euler-identity}

For all $\theta \in \R$ it holds
$$
e^{i \theta}=\cos (\theta)+ i \sin (\theta) \,.
$$

:::



::: Theorem 
For all $\theta \in \R$ it holds
$$
\left|e^{i \theta}\right|=1 \,.
$$

:::




::: Theorem

Let $z \in \C$ with $z = x+iy$ and $z \neq 0$. Then
$$
z = \rho e^{i\theta}\,,
$$
where 
$$
\rho := |z| =  \sqrt{x^2 + y^2} \,, \qquad 
\theta := \arg(z) \,.
$$

:::




::: Definition 
### Exponential form

The **exponential form** of a complex number $z \in \C$ is 
$$
z= \rho e^{i\theta} = |z| \, e^{i \arg(z)}  \,.
$$

:::



::: {.Example #example-exponential-form}

**Question.** Write the number 
$$
z=-2+2 i
$$ 
in exponential form.

**Solution.** From Example \ref{example-trigonometric-form} we know that $z = -2+2i$
can be written in trigonometric form as
$$
z = \sqrt{8}  \left[ \cos \left( \frac{3}{4} \pi \right) + i \sin \left( \frac{3}{4} \pi \right)   \right] \,.
$$
By Euler's identity we hence obtain the exponential form
$$
z=\sqrt{8} e^{i \frac{3}{4} \pi} \,.
$$
:::


::: Remark
### Periodicity of exponential

For all $k \in \Z$ we have
$$
e^{i \theta}=e^{i(\theta+2 \pi k)} \,,
$${#eq-exponential-periodic}
meaning that the complex exponential is $2\pi$-periodic.


:::



::: {.Proposition #proposition-complex-exponential}

Let $z, z_1,z_2 \in \C$ and suppose that
$$
z= \rho e^{i \theta} \,, \quad 
z_1 = \rho_1 e^{i \theta_1}\,, \quad 
z_2 = \rho_2 e^{i \theta_2}\,.
$$
We have
$$
z_1 \cdot z_2 = \rho_1 \rho_2 e^{i (\theta_1 + \theta_2)}  \,, \quad 
z^n = \rho^n  e^{i n \theta} \,,
$$
for all $n \in \N$.
:::


::: Example 

**Question.** Compute $(-2+2 i)^{4}$.

**Solution.** We have two possibilities:

1. Use the binomial theorem:
\begin{align*}
(-2+2 i)^{4} & =(-2)^{4}+\left(\begin{array}{l}
4 \\
1
\end{array}\right)(-2)^{3} \cdot 2 i+\left(\begin{array}{l}
4 \\
2
\end{array}\right)(-2)^{2} \cdot(2 i)^{2} \\
& \quad +\left(\begin{array}{l}
4 \\
3
\end{array}\right)(-2) \cdot(2 i)^{3}+(2 i)^{4} \\
& =16-4 \cdot 8 \cdot 2 i-6 \cdot 4 \cdot 4+4 \cdot 2 \cdot 8 i+16 \\
& =16-64 i-96+64 i+16=-64 \,.
\end{align*}

2. A much simpler calculation is possible by using the exponential form: We know that
$$
-2+2 i = \sqrt{8} e^{i \frac{3}{4} \pi} 
$$
by Example \ref{example-exponential-form}. Hence
$$
(-2+2 i)^{4}=\left(\sqrt{8} e^{i \frac{3}{4} \pi}\right)^{4}=8^{2} e^{i 3 \pi}=-64 \,,
$$
where we used that 
$$
e^{i 3 \pi} = e^{i \pi} = \cos(\pi) + i \sin(\pi) = - 1
$$
by $2\pi$ periodicity of $e^{i\theta}$ and Euler's identity. 
:::


::: Definition
### Complex exponential

The complex exponential of $z = a + ib \in \C$ is defined as
$$
e^z = e^a e^{ib}  \,.
$$

:::



::: Theorem

Let $z,w \in \C$. Then
$$
e^{z+w} = e^z e^w \,, \quad (e^z)^{w} = e^{zw} \,.
$${#eq-complex-exponential}

:::




::: Example 

**Question.** Compute $i^{i}$.

**Solution.** We know that 
$$
|i| = 1 \,, \quad \arg(i) = \frac{\pi}{2} \,.
$$
Hence we can write $i$ in exponential form
$$
i= |i| e^{i\arg(i)} = e^{i \frac{\pi}{2}} \,.
$$ 
Therefore
$$
i^{i}=\left(e^{i \frac{\pi}{2}}\right)^{i}=e^{i^2\frac{\pi}{2}}=e^{-\frac{\pi}{2}} \,.
$$

:::



## Fundamental Theorem of Algebra


::: Theorem 
### Fundamental theorem of algebra   {#theorem-fta}

Let $p_{n}(z)$ be a polynomial of degree $n$ with complex coefficients, i.e.,
$$
p_{n}(z)=a_{n} z^{n}+a_{n-1} z^{n-1}+\ldots+a_{1} z+a_{0},
$$
for some coefficients $a_{n}, \ldots, a_{0} \in \C$ with $a_{n} \neq 0$. There exist 
$$
z_{1}, \ldots, z_{n} \in \C
$$ 
solutions to the polynomial equation
$$
p_n(z) = a_{n} z^{n}+a_{n-1} z^{n-1}+\ldots+a_{1} z+a_{0}=0 \,.
$${#eq-fta}
In particular, $p_n$ factorizes as
$$
p_{n}(z)=a_{n}\left(z-z_{1}\right)\left(z-z_{2}\right) \cdots\left(z-z_{n}\right) \,.
$${#eq-fta-0}


:::



::: Example 

**Question.** Find all the complex solutions to
$$
z^{2}=-1
$${#eq-fta-example-1}

**Solution.** The equation $z^2 = -1$ is equivalent to
$$
p(z) = 0 \,, \quad p(z):=z^{2}+1  \,.
$$
Since $p$ has degree $n=2$, the Fundamental Theorem of Algebra tells us that there are two solutions to (@eq-fta-example-1). We have already seen that these two solutions are $z=i$ and $z=-i$. Then $p$ factorizes as
$$
p(z) = z^{2} + 1 = (z-i)(z+i) \,.
$$
:::


::: {.Example   #example-degree-4}

**Question.** Find all the complex solutions to
$$
z^{4}-1=0 \,.
$${#eq-fta-example-2}

**Solution** The associated polynomial equation is 
$$
p(z) = 0 \,, \quad p(z) := z^4 - 1 \,. 
$$
Since $p$ has degree $n=4$, the Fundamental Theorem of Algebra tells us that there are $4$ solutions to (@eq-fta-example-2). Let us find such solutions. We use the well known identity
$$
a^2-b^2 = (a+b)(a-b) \,, \quad \forall \, a,b \in \R \,,
$$
to factorize $p$. We get:
$$
p(z) = (z^4-1) = (z^2+1)(z^2-1) \,.
$$
We know that 
$$
z^2 + 1 = 0 
$$
has solutions $z = \pm i$. Instead  
$$
z^2 - 1 = 0 
$$
has solutions $x = \pm 1$. Hence, the four solutions of (@eq-fta-example-2) are given by 
$$
z=1,-1, i,-i \,,
$$
and $p$ factorizes as
$$
p(z) = z^4 - 1 = (z-1)(z+1)(z-i)(z+i) \,.
$$

:::


::: Definition
### Multiplicity

Suppose that the polynomial $p_n$ factorizes as 
$$
p_n(z) = a_n (z-z_1)^{k_1} (z-z_2)^{k_2} \cdots (z-z_m)^{k_m} 
$$
with $a_n \neq 0$, $z_1,\ldots, z_m \in \C$ and $k_1, \ldots , k_m \in \N$, $k_i \geq 1$. In this case $p_n$ has degree
$$
n = k_1 + \ldots + k_m = \sum_{i=1}^m k_i \,.
$$
Note that $z_i$ is solves the equation
$$
p_n(z) = 0
$$
exactly $k_i$ times. We call $k_i$ the **multiplicity** of the solution $z_i$.
:::

::: {.Example  #example-multiplicity}

The equation
$$
(z-1)(z-2)^{2}(z+i)^{3}=0
$$
has 6 solutions: 

- $z=1$ with multiplicity $1$
- $z=2$ with multiplicity $2$ 
- $z=-i$ with multiplicity $3$

:::




## Solving polynomial equations



::: Proposition
### Quadratic formula    {#proposition-quadratic-formula}

Let $a, b, c \in \R, a \neq 0$ and consider the equation
$$
ax^2 + bx + c = 0 \,.
$${#eq-quadratic-formula}
Define 
$$
\Delta := b^2 - 4 ac \in \R \,.
$$
The following hold:

1. If $\Delta > 0$ then (@eq-quadratic-formula) has two distinct real solutions $z_1,z_2 \in \R$ given by
$$
z_1 = \frac{-b - \sqrt{\Delta}}{2 a} \,, 
\quad 
z_2 = \frac{-b + \sqrt{\Delta}}{2 a} \,.
$$
2. If $\Delta = 0$ then (@eq-quadratic-formula) has one real solution $z \in \R$ with multiplicity $2$. Such solution is given by
$$
z = z_1 = z_2 = \frac{-b}{2 a} \,.
$$
3. If $\Delta < 0$ then (@eq-quadratic-formula) has two distinct complex solutions $z_1,z_2 \in \C$ given by 
$$
z_1 = \frac{-b - i\sqrt{-\Delta}}{2 a} \,, 
\quad 
z_2 = \frac{-b + i\sqrt{-\Delta}}{2 a} \,,
$$
where $\sqrt{-\Delta} \in \R$, since $-\Delta>0$.

In all cases, the polynomial at (@eq-quadratic-formula) factorizes as
$$
a z^{2}+b z+c = a (z-z_1)(z-z_2) \,.
$$

:::




::: Example 


**Question.** Solve the following equations:

1. $3 z^{2}-6 z+2 = 0$
2. $4 z^{2}-8 z+4=0$
3. $z^{2}+2 z+3=0$

**Solution.**

1. We have that
$$
\Delta = (-6)^{2}-4 \cdot 3 \cdot 2 = 12 > 0
$$
Therefore the equation has two distinct real solutions, given by
$$
z=\frac{-(-6) \pm \sqrt{12}}{2 \cdot 3}=\frac{6 \pm \sqrt{12}}{6}=1 \pm \frac{\sqrt{3}}{3}
$$
In particular we have the factorization
$$
3 z^{2}-6 z+2  = 3 \left( z - 1 - \frac{\sqrt{3}}{3} \right) \left( z - 1 + \frac{\sqrt{3}}{3} \right) \,.
$$



2. We have that 
$$
\Delta = (-8)^{2}-4 \cdot 4 \cdot 4 = 0 \,.
$$
Therefore there exists one solution with multiplicity $2$. This
is given by
$$
z=\frac{-(-8)}{2 \cdot 4} = 1 \,.
$$
In particular we have the factorization
$$
4 z^{2}-8 x+4 = 4 (z-1)^2 \,.
$$



3. We have
$$
\Delta = 2^{2}-4 \cdot 1 \cdot 3 = - 8 < 0 \,.
$$
Therefore there are two complex solutions given by
$$
z=\frac{-2 \pm i \sqrt{8}}{2 \cdot 1} = -1 \pm i \sqrt{2}  \,.
$$
In particular we have the factorization
$$
z^{2}+2 z+3 = (z + 1 - i \sqrt{2}) (z + 1 + i\sqrt{2}) \,.
$$

:::


::: Proposition   
### Quadratic formula with complex coefficients {#proposition-quadratic-formula-C}

Let $a, b, c \in \C, a \neq 0$. The two solutions to 
$$
a z^{2}+b z + c=0
$$ 
are given by
$$
z_1 = \frac{-b + S_1}{2 a} \,, 
\quad 
z_2 = \frac{-b + S_2}{2 a} \,, 
$$
where $S_1$ and $S_2$ are the two solutions to
$$
z^2 = \Delta \,, \quad \Delta := b^2 - 4ac \,.
$$

:::





::: Example

**Question** Find all the solutions to
$$
\frac{1}{2} z^{2}-(3+i) z+(4-i)=0 \,.
$${#eq-example-complex-delta}

**Solution.** We have
\begin{align*}
\Delta & = (-(3+i))^{2}-4 \cdot \frac{1}{2} \cdot(4-i) \\
       & = 8+6 i-8+2 i \\
       & =8 i \,.
\end{align*}
Therefore $\Delta \in \C$. We have to find solutions $S_1$ and $S_2$ to the equation
$$
z^2 = \Delta = 8i \,.
$${#eq-example-complex-delta-2}
We look for solutions of the form $z=a+ i b$. Then we must have that
$$
z^{2}=(a+ ib)^{2}=a^{2}-b^{2}+2 a b i = 8 i \,.
$$
Thus
$$
a^{2}-b^{2}=0 \,, \quad 2 a b = 8  \,.
$$ 
From the first equation we conclude that $|a|=|b|$. From the second equation we have that $ab=4$, and therefore $a$ and $b$ must have the same sign. Hence $a=b$, and 
$$
2 a b = 8 \quad \implies \quad a = b = \pm 2 \,.
$$
From this we conclude that the solutions to (@eq-example-complex-delta-2)
are 
$$
S_{1} = 2+2 i \,, \quad  S_{2}=-2-2 i \,. 
$$
 Hence the solutions to (@eq-example-complex-delta) are
\begin{align*}
z_1 & = \frac{3+i+S_{1}}{2 \cdot \frac{1}{2}}  = 3 + i + S_{1} \\
    & = 3 + i + 2 + 2i = 5 + 3i \,, 
\end{align*}
and 
\begin{align*}
z_2 & = \frac{3+i+S_{2}}{2 \cdot \frac{1}{2}}  = 3+i+S_{2} \\
    & = 3+i -2 - 2i  = 1 - i \,. 
\end{align*}
In particular, the given polynomial factorizes as
\begin{align*}
\frac{1}{2} z^{2}-(3+i) z+(4-i) & = \frac12 (z - z_1)(z-z_2) \\
                                & = \frac12 (z - 5 - 3i)(z - 1 + i) \,. 
\end{align*}

:::



::: Example 

**Question.** Consider the equation
$$
z^{3}-7 z^{2}+6 z=0 \,.
$$ 

1. Check whether $z=0,1,-1$ are solutions.
2. Using your answer from Point 1, and polynomial division, find all the solutions.

**Solution.**

1. By direct inspection we see that $z=0$ and $z=1$ are solutions.

2. Since $z = 0$ is a solution, we can factorize
$$
z^{3}-7 z^{2}+6 z=z\left(z^{2}-7 z+6\right) \,.
$$
We could now use the quadratic formula on the term $z^{2}-7 z+6$ to find the remaining two roots. However, we have already observed that $z=1$ is a solution. Therefore $z-1$ divides $z^{2}-7 z+6$. Using polynomial long division, see @fig-polynomial, we find that
$$
\frac{z^{2}-7 z+6}{z-1}=z-6 \,.
$$
Therefore the last solution is $z=6$, and
$$
z^{3}-7 z^{2}+6 z=z(z-1)(z-6) \,.
$$

:::

![Polynomial long division between $z^{2}-7 z+6$ and $z-1$.](/images/polynomial_1.png){#fig-polynomial width=20%}



::: Example

**Question.** Find all the complex solutions to
$$
z^{3}-7 z+6=0 \,.
$$ 

**Solution.** It is easy to see $z=1$ is a solution. This means that $z-1$ divides $z^{3}-7 z+6$. By using polynomial long division, see @fig-polynomial-1, we compute that
$$
\frac{z^{3}-7 z+6}{z-1}=z^{2}+z-6 \,.
$$
We are now left to solve
$$
z^{2}+z-6 = 0\,.
$$
Using the quadratic formula, we see that the above is solved by $z=2$ and $z=-3$.
Therefore the given polynomial factorizes as
$$
z^{3}-7 z+6 = (z-1)(z-2)(z+3) \,.
$$

:::

![Polynomial long division between $z^{3}-7 z+6$ and $z-1$.](/images/polynomial_2.png){#fig-polynomial-1 width=20%}




## Roots of unity

::: Theorem

Let $n \in \N$ and consider the equation
$$
z^{n}=1 \,.
$${#eq-root-unity-1}
All the $n$ solutions to (@eq-root-unity-1) are given by
$$
z_k = \exp \left(i \frac{2 \pi k}{n}\right) \,, \quad k = 0, \ldots, n-1 \,,
$$
where $\exp(x)$ denotes $e^x$.

:::


::: Definition 

The $n$ solutions to 
$$
z^{n}=1
$$ 
are called the **roots of unity**.

:::


::: Example 

**Question.** Find all the solutions to
$$
z^{4}=1 \,.
$$ 

**Solution.** The $4$ solutions are given by
$$
z_k = \exp \left(i \frac{2 \pi k}{4} \right) = \exp \left(i \frac{\pi k}{2} \right)  \,,
$$
for $k=0,1,2,3$. We compute:
\begin{align*}
z_0 & = e^{i 0} = 1 \,, & \quad & z_1 = e^{i \frac{\pi}{2}}=i \,, \\ 
z_2 & = e^{i \pi}=-1 \,, & \quad & z_3 = e^{i \frac{3 \pi}{2}}=-i \, .
\end{align*}
Note that for $k=4$ we would again get the solution $z=e^{i 2 \pi}=1$.

:::


::: Example 

**Question.** Find all the solutions to 
$$
z^{3}=1 \,.
$$ 

**Solution.** The $3$ solutions are given by
$$
z_k = \exp \left( i \frac{2 \pi k}{3} \right) \,,
$$
for $k=0,1,2$. We compute:
$$
z_0=e^{i 0}=1, \quad z_1=e^{i \frac{2 \pi}{3}}, \quad z_2=e^{i \frac{4 \pi}{3}} .
$$
We can write $z_1$ and $z_2$ in cartesian form:
$$
z_1 = e^{i \frac{2 \pi}{3}}=\cos \left(\frac{2 \pi}{3}\right)+i \sin \left(\frac{2 \pi}{3}\right)=-\frac{1}{2}+\frac{\sqrt{3}}{2} i
$$
and
$$
z_2 = e^{i \frac{4 \pi}{3}}=\cos \left(\frac{4 \pi}{3}\right)+i \sin \left(\frac{4 \pi}{3}\right)=-\frac{1}{2}-\frac{\sqrt{3}}{2} i \,.
$$

:::



## Roots in $\C$



::: Theorem

Let $n \in \N$, $c \in \C$ and consider the equation
$$
z^{n}=c \,.
$${#eq-root-C}
All the $n$ solutions to (@eq-root-C) are given by
$$
z_k = \sqrt[n]{|c|} \, \exp \left(i \, \frac{\theta + 2 \pi k}{n}\right) \,, \quad k = 0, \ldots, n-1 \,,
$$
where $\sqrt[n]{|c|}$ is the $n$-th root of the real number $|c|$, and $\theta = \arg(c)$.

:::


::: Example

**Question.** Find all the $z \in \C$ such that
$$
z^{5}=-32 \,.
$$

**Solution.** Let $c = -32$. We have
$$
|c| = |-32|=32=2^{5}\,, \quad \theta = \arg (-32)=\pi \,.
$$ 
The $5$ solutions are given by
$$
z_k =  \left(2^{5}\right)^{\frac{1}{5}} \exp \left(i \pi \, \frac{1+2 k}{5} \right) \,, \quad k \in \Z \,,
$$
for $k=0,1,2,3,4$. We get
\begin{align*}
z_0 & = 2 e^{i \frac{\pi}{5}} \,  & \quad & z_1 = 2 e^{i \frac{3 \pi}{5}}  \\ 
z_2 & = 2 e^{i \pi}=-2 \,  & \quad & z_3=2 e^{i \frac{7 \pi}{5}}  \\
z_4 &= 2 e^{i \frac{9 \pi}{5}}  & \quad & 
\end{align*}

:::


::: Example 

**Question.** Find all the $z \in \C$ such that
$$
z^{4}=9\left(\cos \left(\frac{\pi}{3}\right)+i \sin \left(\frac{\pi}{3}\right)\right) \,.
$$

**Solution.** Set 
$$
c:=9\left(\cos \left(\frac{\pi}{3}\right)+i \sin \left(\frac{\pi}{3}\right)\right) \,.
$$
The complex number $c$ is already in the trigonometric form, so that we can immediately obtain
$$
|c| = 9 \,, \quad \theta = \arg(c) = \frac{\pi}{3} \,.
$$
The $4$ solutions are given by
\begin{align*}
z_k & = \sqrt[4]{9} \, \exp \left( i \,  \frac{ \pi/3 + 2 \pi k}{4} \right) \\
& = \sqrt{3} \exp \left(  i \pi \, \frac{1+6 k}{12} \right) 
\end{align*}
for $k=0,1,2,3$. We compute
\begin{align*}
z_0 & = \sqrt{3} e^{i \pi \frac{1}{12}} & \quad & z_1 = \sqrt{3} e^{i \pi \frac{7}{12}} \\
z_2 & = \sqrt{3} e^{i \pi \frac{13}{12}}  & \quad &  z_3 = \sqrt{3} e^{i \pi \frac{19}{12}} 
\end{align*}

:::



